bedrock2/src/bedrock2Examples/ARPResponder_live_packet_predicates_on_bytelists.v
@@ -1,0 +1,304 @@
+Require Import Coq.derive.Derive.
+Require Import coqutil.Z.Lia.
+Require coqutil.Word.BigEndian.
+Require Import coqutil.Byte coqutil.Datatypes.HList.
+Require Import coqutil.Tactics.letexists coqutil.Tactics.Tactics coqutil.Tactics.rewr.
+Require Import coqutil.Map.Interface coqutil.Map.Properties.
+Require Import coqutil.Word.Interface coqutil.Word.Properties.
+Require Import bedrock2.Syntax bedrock2.Semantics.
+Require Import bedrock2.NotationsCustomEntry coqutil.Z.HexNotation.
+Require Import bedrock2.FE310CSemantics.
+Require Import bedrock2.Map.Separation bedrock2.Map.SeparationLogic bedrock2.Array.
+Require Import bedrock2.ZnWords.
+Require Import bedrock2.WeakestPrecondition bedrock2.ProgramLogic.
+
+Section WithParameters.
+  Context {p : FE310CSemantics.parameters}.
+  Import Syntax BinInt String List.ListNotations ZArith.
+  Local Set Implicit Arguments.
+  Local Open Scope string_scope. Local Open Scope Z_scope. Local Open Scope list_scope.
+  Local Coercion expr.literal : Z >-> expr.
+  Local Coercion expr.var : String.string >-> expr.
+  Infix "\*" := sep (at level 45, right associativity).
+
+  (* ** Packet Formats *)
+
+  Inductive EtherType := EtherTypeARP | EtherTypeIPv4.
+
+  Definition encodeEtherType(t: EtherType): list byte :=
+    match t with
+    | EtherTypeARP => [Byte.x08; Byte.x06]
+    | EtherTypeIPv4 => [Byte.x08; Byte.x00]
+    end.
+
+  Definition MAC := tuple byte 6.
+
+  Definition encodeMAC: MAC -> list byte := tuple.to_list.
+
+  Definition IPv4 := tuple byte 4.
+
+  Definition encodeIPv4: IPv4 -> list byte := tuple.to_list.
+
+  Definition encodeCRC(crc: Z): list byte := tuple.to_list (BigEndian.split 4 crc).
+
+  Record EthernetPacket(Payload: Type) := mkEthernetARPPacket {
+    dstMAC: MAC;
+    srcMAC: MAC;
+    etherType: EtherType;
+    payload: Payload;
+  }.
+
+  (* Note: At the moment we want to allow any padding and crc, so we use an isXxx predicate rather
+     than an encodeXxx function *)
+  Definition isEthernetPacket{P: Type}(payloadOk: P -> list byte -> Prop)(p: EthernetPacket P)(bs: list byte) :=
+    exists data padding crc,
+      bs = encodeMAC p.(srcMAC) ++ encodeMAC p.(dstMAC) ++ encodeEtherType p.(etherType)
+           ++ data ++ padding ++ encodeCRC crc /\
+      payloadOk p.(payload) data /\
+      46 <= Z.of_nat (List.length (data ++ padding)) <= 1500.
+      (* TODO could/should also verify CRC *)
+
+  Inductive ARPOperation := ARPOperationRequest | ARPOperationReply.
+
+  Definition encodeARPOperation(oper: ARPOperation): list byte :=
+    match oper with
+    | ARPOperationRequest => [Byte.x01]
+    | ARPOperationReply => [Byte.x02]
+    end.
+
+  Record ARPPacket := mkARPPacket {
+    oper: ARPOperation;
+    sha: MAC;  (* sender hardware address *)
+    spa: IPv4; (* sender protocol address *)
+    tha: MAC;  (* target hardware address *)
+    tpa: IPv4; (* target protocol address *)
+  }.
+
+  Definition encodeARPPacket(p: ARPPacket): list byte :=
+    [
+      Byte.x00; Byte.x01; (* hardware type: Ethernet *)
+      Byte.x80; Byte.x00; (* protocol type *)
+      Byte.x06;           (* hardware address length (6 for MAC addresses) *)
+      Byte.x04            (* protocol address length (4 for IPv4 addresses) *)
+    ] ++ encodeARPOperation p.(oper)
+    ++ encodeMAC p.(sha) ++ encodeIPv4 p.(spa) ++ encodeMAC p.(tha) ++ encodeIPv4 p.(tpa).
+
+  Definition isEthernetARPPacket: EthernetPacket ARPPacket -> list byte -> Prop :=
+    isEthernetPacket (fun arpP => eq (encodeARPPacket arpP)).
+
+  Record ARPConfig := mkARPConfig {
+    myMAC: MAC;
+    myIPv4: IPv4;
+  }.
+
+  Context (cfg: ARPConfig).
+
+  (* high-level protocol definition (does not mention lists of bytes) *)
+  Definition ARPReqResp(req resp: EthernetPacket ARPPacket): Prop :=
+    req.(etherType) = EtherTypeARP /\
+    req.(payload).(oper) = ARPOperationRequest /\
+    req.(payload).(tpa) = cfg.(myIPv4) /\ (* <-- we only reply to requests asking for our own MAC *)
+    resp.(dstMAC) = req.(payload).(sha) /\
+    resp.(srcMAC) = cfg.(myMAC) /\
+    resp.(etherType) = EtherTypeARP /\
+    resp.(payload).(oper) = ARPOperationReply /\
+    resp.(payload).(sha) = cfg.(myMAC) /\ (* <-- the actual reply *)
+    resp.(payload).(spa) = cfg.(myIPv4) /\
+    resp.(payload).(tha) = req.(payload).(sha) /\
+    resp.(payload).(tpa) = req.(payload).(spa).
+
+  Lemma length_encodeARPOperation: forall op, List.length (encodeARPOperation op) = 1%nat.
+  Proof. intros. destruct op; reflexivity. Qed.
+
+  Lemma length_encodeEtherType: forall et, List.length (encodeEtherType et) = 2%nat.
+  Proof. intros. destruct et; reflexivity. Qed.
+
+  Fixpoint firstn_as_tuple{A: Type}(default: A)(n: nat)(l: list A): tuple A n :=
+    match n as n return tuple A n with
+    | O => tt
+    | S m => PrimitivePair.pair.mk (List.hd default l) (firstn_as_tuple default m (List.tl l))
+    end.
+
+  Lemma to_list_firstn_as_tuple: forall A (default: A) n (l: list A),
+      (n <= List.length l)%nat ->
+      tuple.to_list (firstn_as_tuple default n l) = List.firstn n l.
+  Proof.
+    induction n; intros.
+    - reflexivity.
+    - destruct l. 1: cbv in H; exfalso; blia.
+      simpl in *.
+      f_equal. eapply IHn. blia.
+  Qed.
+
+  Lemma to_list_BigEndian_split: forall n (l: list byte),
+      (n <= List.length l)%nat ->
+      tuple.to_list (BigEndian.split n (BigEndian.combine n (firstn_as_tuple Byte.x00 n l))) = List.firstn n l.
+  Proof.
+    intros. rewrite BigEndian.split_combine.
+    apply to_list_firstn_as_tuple.
+    assumption.
+  Qed.
+
+  Lemma list_eq_cancel_step{A: Type}: forall (xs ys l: list A),
+    List.firstn (List.length xs) l = xs ->
+    List.skipn (List.length xs) l = ys ->
+    l = xs ++ ys.
+  Proof.
+    intros. remember (List.length xs) as n. subst xs ys. symmetry. apply List.firstn_skipn.
+  Qed.
+
+  Lemma list_eq_cancel_firstn: forall A (l rest: list A) n,
+      (n <= List.length l)%nat ->
+      List.skipn n l = rest ->
+      l = List.firstn n l ++ rest.
+  Proof. intros. subst rest. symmetry. apply List.firstn_skipn. Qed.
+
+  Ltac length_getEq t :=
+    match t with
+    | context[List.length (tuple.to_list ?xs)] => constr:(tuple.length_to_list xs)
+    | context[List.length (?xs ++ ?ys)] => constr:(List.app_length xs ys)
+    | context[List.length (?x :: ?xs)] => constr:(List.length_cons x xs)
+    | context[List.length (@nil ?A)] => constr:(@List.length_nil A)
+    | context[List.skipn ?n (List.skipn ?m ?xs)] => constr:(List.skipn_skipn n m xs)
+    | context[List.length (encodeEtherType ?et)] => constr:(length_encodeEtherType et)
+    | context[List.length (encodeARPOperation ?op)] => constr:(length_encodeARPOperation op)
+    | context[List.length (List.skipn ?n ?l)] => constr:(List.skipn_length n l)
+    end.
+
+  Lemma list_instantiate_evar{A: Type}: forall l1 l2 l3 (xs1 xs3 evar lhs rhs: list A),
+      (* reshape rhs: *)
+      rhs = xs1 ++ evar ++ xs3 ->
+      (* equations for lengths l1, l2, l3 *)
+      l1 = List.length xs1 ->
+      l2 = (List.length lhs - l1 - l3)%nat ->
+      l3 = List.length xs3 ->
+      (* sidecondition on lengths *)
+      (l1 + l3 <= List.length lhs)%nat ->
+      (* equations for lists xs1, evar, xs3 *)
+      xs1 = List.firstn l1 lhs ->
+      evar = List.firstn (List.length lhs - l1 - l3) (List.skipn l1 lhs) ->
+      xs3 = List.skipn (List.length lhs - l3) lhs ->
+      lhs = rhs.
+  Proof.
+    intros. subst xs1 xs3 evar. subst rhs.
+    apply list_eq_cancel_step. {
+      f_equal. symmetry. assumption.
+    }
+    apply list_eq_cancel_step. {
+      rewrite <- H0. f_equal. rewrite List.length_firstn_inbounds. 1: reflexivity.
+      rewrite List.length_skipn.
+      blia.
+    }
+    rewr length_getEq in |-*.
+    f_equal.
+    rewrite List.length_firstn_inbounds.
+    1: blia.
+    rewrite List.length_skipn.
+    blia.
+  Qed.
+
+  Lemma instantiate_tuple_from_list{A: Type}: forall (n: nat) (evar: tuple A n) (l: list A) (default: A),
+      n = Datatypes.length l ->
+      evar = firstn_as_tuple default n l ->
+      tuple.to_list evar = l.
+  Proof.
+    intros. subst.
+    rewrite to_list_firstn_as_tuple. 2: reflexivity.
+    apply List.firstn_all2. reflexivity.
+  Qed.
+
+  Ltac list_eq_cancel_step :=
+    apply list_eq_cancel_step;
+    (* can't use normal rewrite because COQBUG https://github.com/coq/coq/issues/10848 *)
+    rewr length_getEq in |-*.
+
+  Definition TODO{T: Type}: T. Admitted.
+
+  Lemma interpretEthernetARPPacket: forall bs,
+      Z.of_nat (List.length bs) = 64 ->
+      (* conditions collected while trying to prove the lemma: *)
+      List.firstn 2 (List.skipn 12 bs) = [Byte.x08; Byte.x06] ->
+      List.firstn 6 (List.skipn 14 bs) = [Byte.x00; Byte.x01; Byte.x80; Byte.x00; Byte.x06; Byte.x04] ->
+      List.firstn 1 (List.skipn 20 bs) = [Byte.x01] -> (* we only interpret requests at the moment, no replies *)
+      exists packet: EthernetPacket ARPPacket, isEthernetARPPacket packet bs.
+  Proof.
+    intros.
+    unfold isEthernetARPPacket, isEthernetPacket, encodeARPPacket, encodeMAC, encodeIPv4, encodeCRC.
+    eexists ({| payload := {| oper := _ |} |}).
+    cbn [dstMAC srcMAC etherType payload oper sha spa tha tpa].
+    repeat eexists.
+    (* can't use normal rewrite because COQBUG https://github.com/coq/coq/issues/10848 *)
+    all: rewr (fun t => match t with
+           | context [ List.length (?xs ++ ?ys) ] => constr:(List.app_length xs ys)
+           | context [ List.length (encodeARPOperation ?op) ] => constr:(length_encodeARPOperation op)
+           | context [ List.length (?h :: ?t) ] => constr:(List.length_cons h t)
+           | context [ (?xs ++ ?ys) ++ ?zs ] => constr:(eq_sym (List.app_assoc xs ys zs))
+           end) in |-*.
+    {
+      list_eq_cancel_step. {
+        symmetry. apply to_list_firstn_as_tuple with (default := Byte.x00). ZnWords.
+      }
+      list_eq_cancel_step. {
+        symmetry. apply to_list_firstn_as_tuple with (default := Byte.x00). ZnWords.
+      }
+      list_eq_cancel_step. {
+        instantiate (1 := EtherTypeARP).
+        assumption.
+      }
+      list_eq_cancel_step. {
+        assumption.
+      }
+      list_eq_cancel_step. {
+        instantiate (1 := ARPOperationRequest).
+        assumption.
+      }
+      list_eq_cancel_step. {
+        symmetry. apply to_list_firstn_as_tuple with (default := Byte.x00). ZnWords.
+      }
+      list_eq_cancel_step. {
+        symmetry. apply to_list_firstn_as_tuple with (default := Byte.x00). ZnWords.
+      }
+      list_eq_cancel_step. {
+        symmetry. apply to_list_firstn_as_tuple with (default := Byte.x00). ZnWords.
+      }
+      list_eq_cancel_step. {
+        symmetry. apply to_list_firstn_as_tuple with (default := Byte.x00). ZnWords.
+      }
+      cbn -[List.skipn tuple.to_list].
+      eapply list_instantiate_evar with (xs1 := nil). {
+        cbn [List.app].
+        f_equal.
+      }
+      { cbn [List.length]. reflexivity. }
+      { reflexivity. }
+      { reflexivity. }
+      { rewrite tuple.length_to_list. rewrite List.length_skipn. blia. }
+      { reflexivity. }
+      { (* finally, we can "automatically" instantiate the evar ?padding *)
+        reflexivity.  }
+      rewr length_getEq in |-*.
+      rewrite BigEndian.split_combine.
+      etransitivity. 2: apply tuple.to_list_of_list.
+      match goal with
+      | |- @tuple.to_list _ ?n1 _ = @tuple.to_list _ ?n2 _ =>
+        replace n2 with n1 by (rewr length_getEq in |-*; blia)
+      end.
+      eapply instantiate_tuple_from_list with (default := Byte.x00). 2: reflexivity.
+      rewr length_getEq in |-*.
+      blia.
+    }
+    {
+      rewr length_getEq in |-*.
+      rewrite List.firstn_length.
+      rewr length_getEq in |-*.
+      blia.
+    }
+    {
+      rewr length_getEq in |-*.
+      rewrite List.firstn_length.
+      rewr length_getEq in |-*.
+      blia.
+    }
+  Qed.
+
+End WithParameters.
